distributed lockServer without dedicated ownership invariants

messageInvariantPrototypes/lockServer/distributed/applicationProof.dfy
@@ -1,9 +1,11 @@
-include "spec.dfy"
+include "messageInvariants.dfy"
 
-module OwnershipInvariants {
+module LockServerProof {
   import opened Types
   import opened UtilitiesLibrary
   import opened DistributedSystem
+  import opened Obligations
+  import opened MessageInvariants
 
 /***************************************************************************************
 *                                   Definitions                                        *
@@ -20,10 +22,10 @@ module OwnershipInvariants {
   {
     && msg in v.network.sentMsgs
     && ((0 <= msg.Dst() < |c.clients| &&
-          ClientHost.UniqueKeyInFlightForHost(c.clients[msg.Dst()], v.Last().clients[msg.Dst()], k, msg)
+          ClientHost.UniqueKeyInFlightForHost(c.clients[msg.Dst()], v.clients[msg.Dst()], k, msg)
         )
         || (0 <= msg.Dst() < |c.server| &&
-            ServerHost.UniqueKeyInFlightForHost(c.server[msg.Dst()], v.Last().server[msg.Dst()], k, msg)
+            ServerHost.UniqueKeyInFlightForHost(c.server[msg.Dst()], v.server[msg.Dst()], k, msg)
         )
     )
   }
@@ -33,7 +35,7 @@ module OwnershipInvariants {
   {
     forall idx | 0 <= idx < |c.clients| 
     :: 
-    !ClientHost.HostOwnsUniqueKey(c.clients[idx], v.Last().clients[idx], k)
+    !ClientHost.HostOwnsUniqueKey(c.clients[idx], v.clients[idx], k)
   }
 
   ghost predicate NoServerOwnsKey(c: Constants, v: Variables, k: UniqueKey) 
@@ -41,7 +43,7 @@ module OwnershipInvariants {
   {
     forall idx | 0 <= idx < |c.server|
     :: 
-    !ServerHost.HostOwnsUniqueKey(c.server[idx], v.Last().server[idx], k)
+    !ServerHost.HostOwnsUniqueKey(c.server[idx], v.server[idx], k)
   }
 
   ghost predicate NoHostOwnsKey(c: Constants, v: Variables, k: UniqueKey) 
@@ -77,8 +79,8 @@ module OwnershipInvariants {
     forall h1, h2, k | 
       && 0 <= h1 < |c.clients|
       && 0 <= h2 < |c.clients|
-      && ClientHost.HostOwnsUniqueKey(c.clients[h1], v.Last().clients[h1], k) 
-      && ClientHost.HostOwnsUniqueKey(c.clients[h2], v.Last().clients[h2], k) 
+      && ClientHost.HostOwnsUniqueKey(c.clients[h1], v.clients[h1], k) 
+      && ClientHost.HostOwnsUniqueKey(c.clients[h2], v.clients[h2], k) 
     ::
       && h1 == h2
   }
@@ -89,8 +91,8 @@ module OwnershipInvariants {
     forall h1, h2, k | 
       && 0 <= h1 < |c.server|
       && 0 <= h2 < |c.server|
-      && ServerHost.HostOwnsUniqueKey(c.server[h1], v.Last().server[h1], k) 
-      && ServerHost.HostOwnsUniqueKey(c.server[h2], v.Last().server[h2], k) 
+      && ServerHost.HostOwnsUniqueKey(c.server[h1], v.server[h1], k) 
+      && ServerHost.HostOwnsUniqueKey(c.server[h2], v.server[h2], k) 
     ::
       && h1 == h2
   }
@@ -106,37 +108,56 @@ module OwnershipInvariants {
   {
     forall k | !NoServerOwnsKey(c, v, k) :: NoClientOwnsKey(c, v, k)
   }
-  
-  
-  ghost predicate OwnershipInv(c: Constants, v: Variables)
+
+  ghost predicate ServerOwnsLockImpliesNoClientsOwnsLock(c: Constants, v: Variables)
+  requires v.WF(c)
   {
-    && v.WF(c)
+    v.server[0].hasLock ==> 
+    (forall id | c.ValidClientIdx(id) :: !v.clients[id].hasLock)
+  }
+  
+  ghost predicate ApplicationInv(c: Constants, v: Variables)
+    requires v.WF(c)
+  {
     && AtMostOneInFlightMessagePerKey(c, v)
     && AtMostOneOwnerPerKeyClients(c, v)
     && AtMostOneOwnerPerKeyServers(c, v)
     && HostOwnsKeyImpliesNotInFlight(c, v)
-    && ClientsOwnKey(c, v)
-    && ServersOwnKey(c, v)
+    && ServerOwnsLockImpliesNoClientsOwnsLock(c, v)
   }
 
-  // Base obligation
-  lemma InitImpliesOwnershipInv(c: Constants, v: Variables)
-    requires Init(c, v)
-    ensures OwnershipInv(c, v)
+  ghost predicate Inv(c: Constants, v: Variables)
+  {
+    && v.WF(c)
+    && MessageInv(c, v)
+    && ApplicationInv(c, v)
+    && Safety(c, v)
+  }
+
+  lemma InvImpliesSafety(c: Constants, v: Variables)
+    requires Inv(c, v)
+    ensures Safety(c, v)
   {}
 
-  // Inductive obligation
-  lemma OwnershipInvInductive(c: Constants, v: Variables, v': Variables)
-    requires OwnershipInv(c, v)
-    requires Next(c, v, v')
-    ensures OwnershipInv(c, v')
+  lemma InitImpliesInv(c: Constants, v: Variables)
+    requires Init(c, v)
+    ensures Inv(c, v)
   {
+    InitImpliesMessageInv(c, v);
+  }
+
+  lemma InvInductive(c: Constants, v: Variables, v': Variables)
+    requires Inv(c, v)
+    requires Next(c, v, v')
+    ensures Inv(c, v')
+  {
+    MessageInvInductive(c, v, v');
     InvNextAtMostOneInFlightMessagePerKey(c, v, v');
     InvNextHostOwnsKeyImpliesNotInFlight(c, v, v');
     InvNextAtMostOwnerPerKeyClients(c, v, v');
     InvNextAtMostOwnerPerKeyServers(c, v, v');
-    InvNextClientsOwnKey(c, v, v');
     InvNextServersOwnKey(c, v, v');
+    AtMostOwnerPerKeyImpliesSafety(c, v');
   }
 
 
@@ -144,10 +165,28 @@ module OwnershipInvariants {
 *                                 InvNext Proofs                                       *
 ***************************************************************************************/
 
+lemma AtMostOwnerPerKeyImpliesSafety(c: Constants, v: Variables)
+  requires v.WF(c)
+  requires AtMostOneOwnerPerKeyClients(c, v)
+  ensures Safety(c, v)
+{
+  forall idx1, idx2 | 
+    && c.ValidClientIdx(idx1) 
+    && c.ValidClientIdx(idx2) 
+    && HoldsLock(c, v, idx1)
+    && HoldsLock(c, v, idx2)
+  ensures
+   idx1 == idx2
+  {
+    // triggers
+    assert ClientHost.HostOwnsUniqueKey(c.clients[idx1], v.clients[idx1], 0);
+    assert ClientHost.HostOwnsUniqueKey(c.clients[idx2], v.clients[idx2], 0);
+  }
+}
 
 lemma InvNextAtMostOneInFlightMessagePerKey(c: Constants, v: Variables, v': Variables)
   requires v'.WF(c)
-  requires OwnershipInv(c, v)
+  requires Inv(c, v)
   requires Next(c, v, v')
   ensures AtMostOneInFlightMessagePerKey(c, v')
 {
@@ -166,7 +205,7 @@ lemma InvNextAtMostOneInFlightMessagePerKey(c: Constants, v: Variables, v': Vari
 
 lemma InvNextAtMostOneInFlightHelper(c: Constants, v: Variables, v': Variables, m1: Message, m2: Message, k: UniqueKey)
   requires v'.WF(c)
-  requires OwnershipInv(c, v)
+  requires Inv(c, v)
   requires Next(c, v, v')
   // input constraints
   requires m1 != m2
@@ -180,7 +219,7 @@ lemma InvNextAtMostOneInFlightHelper(c: Constants, v: Variables, v': Variables, 
 
 lemma InvNextHostOwnsKeyImpliesNotInFlight(c: Constants, v: Variables, v': Variables)
   requires v'.WF(c)
-  requires OwnershipInv(c, v)
+  requires Inv(c, v)
   requires Next(c, v, v')
   ensures HostOwnsKeyImpliesNotInFlight(c, v')
 {
@@ -192,7 +231,7 @@ lemma InvNextHostOwnsKeyImpliesNotInFlight(c: Constants, v: Variables, v': Varia
       if msg in v.network.sentMsgs {
         assert KeyInFlightByMessage(c, v, msg, k);
         assert NoHostOwnsKey(c, v, k);  
-        var dsStep :| NextStep(c, v.Last(), v'.Last(), v.network, v'.network, dsStep);
+        var dsStep :| NextStep(c, v, v', dsStep);
         assert dsStep.msgOps.recv.value == msg by {
           if dsStep.msgOps.recv.value != msg {
             var m' := dsStep.msgOps.recv.value;
@@ -208,26 +247,26 @@ lemma InvNextHostOwnsKeyImpliesNotInFlight(c: Constants, v: Variables, v': Varia
 
 lemma InvNextAtMostOwnerPerKeyClients(c: Constants, v: Variables, v': Variables) 
   requires v'.WF(c)
-  requires OwnershipInv(c, v)
+  requires Inv(c, v)
   requires Next(c, v, v')
   ensures AtMostOneOwnerPerKeyClients(c, v')
 {
   forall h1, h2, k | 
       && 0 <= h1 < |c.clients|
       && 0 <= h2 < |c.clients|
-      && ClientHost.HostOwnsUniqueKey(c.clients[h1], v'.Last().clients[h1], k) 
-      && ClientHost.HostOwnsUniqueKey(c.clients[h2], v'.Last().clients[h2], k) 
+      && ClientHost.HostOwnsUniqueKey(c.clients[h1], v'.clients[h1], k) 
+      && ClientHost.HostOwnsUniqueKey(c.clients[h2], v'.clients[h2], k) 
   ensures
      && h1 == h2
   {
-    var dsStep :| NextStep(c, v.Last(), v'.Last(), v.network, v'.network, dsStep);
+    var dsStep :| NextStep(c, v, v', dsStep);
     if h1 != h2 {
-      if ClientHost.HostOwnsUniqueKey(c.clients[h2], v'.Last().clients[h2], k) {
+      if ClientHost.HostOwnsUniqueKey(c.clients[h2], v'.clients[h2], k) {
         assert KeyInFlightByMessage(c, v, dsStep.msgOps.recv.value, k);  
         assert UniqueKeyInFlight(c, v, k);
         assert false;
       }
-      if ClientHost.HostOwnsUniqueKey(c.clients[h1], v'.Last().clients[h1], k) {
+      if ClientHost.HostOwnsUniqueKey(c.clients[h1], v'.clients[h1], k) {
         assert KeyInFlightByMessage(c, v, dsStep.msgOps.recv.value, k);  
         assert UniqueKeyInFlight(c, v, k);
         assert false;
@@ -238,26 +277,26 @@ lemma InvNextAtMostOwnerPerKeyClients(c: Constants, v: Variables, v': Variables)
 
 lemma InvNextAtMostOwnerPerKeyServers(c: Constants, v: Variables, v': Variables) 
   requires v'.WF(c)
-  requires OwnershipInv(c, v)
+  requires Inv(c, v)
   requires Next(c, v, v')
   ensures AtMostOneOwnerPerKeyServers(c, v')
 {
   forall h1, h2, k | 
       && 0 <= h1 < |c.server|
       && 0 <= h2 < |c.server|
-      && ServerHost.HostOwnsUniqueKey(c.server[h1], v'.Last().server[h1], k) 
-      && ServerHost.HostOwnsUniqueKey(c.server[h2], v'.Last().server[h2], k) 
+      && ServerHost.HostOwnsUniqueKey(c.server[h1], v'.server[h1], k) 
+      && ServerHost.HostOwnsUniqueKey(c.server[h2], v'.server[h2], k) 
   ensures
      && h1 == h2
   {
-    var dsStep :| NextStep(c, v.Last(), v'.Last(), v.network, v'.network, dsStep);
+    var dsStep :| NextStep(c, v, v', dsStep);
     if h1 != h2 {
-      if ServerHost.HostOwnsUniqueKey(c.server[h2], v'.Last().server[h2], k) {
+      if ServerHost.HostOwnsUniqueKey(c.server[h2], v'.server[h2], k) {
         assert KeyInFlightByMessage(c, v, dsStep.msgOps.recv.value, k);  
         assert UniqueKeyInFlight(c, v, k);
         assert false;
       }
-      if ServerHost.HostOwnsUniqueKey(c.server[h1], v'.Last().server[h1], k) {
+      if ServerHost.HostOwnsUniqueKey(c.server[h1], v'.server[h1], k) {
         assert KeyInFlightByMessage(c, v, dsStep.msgOps.recv.value, k);  
         assert UniqueKeyInFlight(c, v, k);
         assert false;
@@ -268,15 +307,15 @@ lemma InvNextAtMostOwnerPerKeyServers(c: Constants, v: Variables, v': Variables)
 
 lemma InvNextClientsOwnKey(c: Constants, v: Variables, v': Variables) 
   requires v'.WF(c)
-  requires OwnershipInv(c, v)
+  requires Inv(c, v)
   requires Next(c, v, v')
   ensures ClientsOwnKey(c, v')
 {
   forall k | !NoClientOwnsKey(c, v', k)
   ensures NoServerOwnsKey(c, v', k) {
-    var dsStep :| NextStep(c, v.Last(), v'.Last(), v.network, v'.network, dsStep);
-    var idx :| 0 <= idx < |c.clients| && ClientHost.HostOwnsUniqueKey(c.clients[idx], v'.Last().clients[idx], k);
-    if ClientHost.HostOwnsUniqueKey(c.clients[idx], v.Last().clients[idx], k) {
+    var dsStep :| NextStep(c, v, v', dsStep);
+    var idx :| 0 <= idx < |c.clients| && ClientHost.HostOwnsUniqueKey(c.clients[idx], v'.clients[idx], k);
+    if ClientHost.HostOwnsUniqueKey(c.clients[idx], v.clients[idx], k) {
       assert !UniqueKeyInFlight(c, v, k);
       if !NoServerOwnsKey(c, v', k) {
         assert KeyInFlightByMessage(c, v, dsStep.msgOps.recv.value, k);
@@ -291,15 +330,15 @@ lemma InvNextClientsOwnKey(c: Constants, v: Variables, v': Variables)
 
 lemma InvNextServersOwnKey(c: Constants, v: Variables, v': Variables) 
   requires v'.WF(c)
-  requires OwnershipInv(c, v)
+  requires Inv(c, v)
   requires Next(c, v, v')
-  ensures ServersOwnKey(c, v')
+  ensures ServerOwnsLockImpliesNoClientsOwnsLock(c, v')
 {
   forall k | !NoServerOwnsKey(c, v', k)
   ensures NoClientOwnsKey(c, v', k) {
-    var dsStep :| NextStep(c, v.Last(), v'.Last(), v.network, v'.network, dsStep);
-    var idx :| 0 <= idx < |c.server| && ServerHost.HostOwnsUniqueKey(c.server[idx], v'.Last().server[idx], k);
-    if ServerHost.HostOwnsUniqueKey(c.server[idx], v.Last().server[idx], k) {
+    var dsStep :| NextStep(c, v, v', dsStep);
+    var idx :| 0 <= idx < |c.server| && ServerHost.HostOwnsUniqueKey(c.server[idx], v'.server[idx], k);
+    if ServerHost.HostOwnsUniqueKey(c.server[idx], v.server[idx], k) {
       assert !UniqueKeyInFlight(c, v, k);
       if !NoClientOwnsKey(c, v', k) {
         assert KeyInFlightByMessage(c, v, dsStep.msgOps.recv.value, k);
@@ -312,4 +351,4 @@ lemma InvNextServersOwnKey(c: Constants, v: Variables, v': Variables)
   }
 }
 
-} // end module ShardedKVProof
+} // end module LockServerProof
